## Propositional Logic (cont.)
*proof*- a sequence of sentences where each sentence

### Rules
**Resolution Rule**
$A\lor B,\neg B\lor C = A\lor C$
$A \lor B, \neg B = A$

**Converting a statement to *Conjunctive Normal Form* (CNF)**
Eliminating the "implies" ($\implies$) and having only conjunctions ($\land$) at the top level of our statement

**Removing implication**
$\alpha \implies \beta = \neg\alpha \lor \beta$

**DeMorgan's Law**
$\neg (\alpha \land \beta) = \neg\alpha\lor\neg\beta$

**Back to statements**
$A \land B$ becomes
1. A
2. B

TODO: add more rules/shortcuts?